---
title: IMO 2024 Selected Solution Sketches
tags: math
---

P1:


Find all real $$\alpha$$ such that for all integers $$n$$,
$$n$$ divides 4 $$\sum_{i = 1}^{n} \lfloor \alpha i \rfloor$$.

$$\alpha$$ has to be an even integer.

Since $$2 \cdot (1 + \ldots n ) = n (n + 1)$$ is divisible by $$n$$,
it suffices to consider the case where $$0 < a < 2$$.

If $$\alpha = 1$$ then $$n = 2$$ fails.

If $$\alpha < 1$$, then there is some $$k \geq 1$$ such that

$$\frac{1}{k + 1}\leq\alpha <\frac{1}{k}$$

Then take $$n = k + 1$$, we get $$0 \ldots 0, 1$$,
whose sum is not divisible by $$(k + 1)$$.

If $$\alpha > 1$$, apply the same argument to $$1 - \alpha$$,
we get the same contradiction for the $$k$$ such that

$$1 - \frac{1}{k} <\alpha\leq 1 - \frac{1}{K + 1}.$$


Formally the terms are like, $$1, 3, 5, \ldots 2k - 3$$,
with last term stricty less than $$2k - 2$$.




P2:

Find all integers $$a$$ and $$b$$
such that there exists $$g$$ and $$N$$ such that for all $$n \geq N$$,
$$(a^{n} + b, b^{n} + a) = g$$.

$$(1, 1)$$ clearly works since every term is just $$2$$.

We claim this is all the solutions possible.

If $$a = b$$, then $$(a^{n} + a, a^{n} + a) = a^{n} + a$$,
so things are never the same.

Otherwise WLOG $$a < b$$.

Consider the number $$ab + 1$$.
We have that for any integer $$k$$,
$$a^{k \cdot \phi\left( ab + 1 \right) }=$$
$$b^{k \cdot \phi\left( ab + 1 \right) }$$
$$\equiv 1 \pmod{\left( a b + 1 \right)}$$

Now consider $$n = k \cdot \phi(ab + 1) - 1$$.
We have
$$a^{k \cdot \phi\left( ab + 1 \right)} + ab=$$
$$1 + ab= 0 \pmod{\left( ab + 1 \right)}$$
or
$$(ab + 1) | (a^{k \cdot \phi(ab + 1)} + ab)$$.
Since $$(a, ab + 1) = 1$$,
we can divide both sides by $$a$$, giving
$$(ab + 1)\mid(a^{n - 1} + b).$$
and similarly
$$(ab + 1)\mid(b^{n - 1} + a).$$

Consider some $$a$$, $$b$$, $$g$$, and $$N$$.

Since $$ab \geq 1$$, $$\phi(ab + 1) \geq 1$$.
So for any $$N$$, we can find $$k$$ such that
$$k \phi(ab + 1) > N$$.

By the above calculation
we get that $$(ab + 1) | g$$.

However, we also get
$$b^{k \phi(ab + 1)} \equiv 1 \pmod{ab + 1}$$
and in turn $$b^{k \phi(ab + 1)} + a \equiv a + 1 \pmod{ab + 1}$$
So we must have $$ab + 1 | a + 1$$.

This can only happen if $$b = 1$$, giving $$a = b = 1$$
as the only solution.

From $$g \mid a^{n} + b$$ and $$g \mid a^{n + 1} + b$$ we get
$$g \mid a^{n + 1} - a^{n},$$
or $$g \mid a^{N} \left( a  - 1 \right). $$


Also since $$(a - b) \mid (a^{n} + b - b^{n} - a)$$,
we get $$(a - b) \mid g$$.

Consider the simplified case where $$g | a$$ and $$g | b$$,
that is, the case where $$g = 1$$.
We then need $$b = a + 1$$, that is, we want to find all $$a$$ such that
$$(a^{n} + a + 1, (a + 1)^{n} + 1) = 1$$
for all $$n \geq N$$.
